RELEASE_NOTES.md
@@ -6,8 +6,10 @@ Modifications in definitions leading to possible incompatibilities with version 
 
 * generalized mix rules
     (no real impact if mix rules are not used except that the `mix0` and `mix2` rules are replaced by a single rule);
-* output of `atomic` is now in `Type` (only requires simple updates if `atomic` is used, it is also possible to use the previous version under the name `atomic_Prop`);
-* results are now parametrized over atom sets (this increases the number of implicit parameters of objects).
+* output of `atomic` is now in `Type` (only requires simple updates if `atomic` is used);
+* results are now parametrized over atom sets (this increases the number of implicit parameters of objects);
+* introduction of `Forall_sequent` to deal with properties of sequents inside proofs rather than `ll_ps` (and similarly for the other systems);
+* parameter `pcut` for cut-rules is now of type `formula -> bool`.
 
 New results added, including:
 
@@ -16,9 +18,16 @@ New results added, including:
 * additional counter-examples to conservativity of `ill` over `ll`;
 * simplified definition of `micro_ll` and new `nano_ll`;
 * decidability of equality on formulas;
-* Girard's translations of intuitionistic logic.
+* Girard's translations of intuitionistic logic;
+* more on focusing (Andreoli's triadic system).
 
-*Tested with Coq v8.13.0.*
+*Tested with Coq v8.17.0.*
+
+## Version 2.0.3 (2022/02/06)
+
+This is mostly an adaptation of v2.0 to Coq v8.15.0 and OLlibs v2.0.2.
+
+*Tested with Coq v8.15.0.*
 
 ## Version 2.0.2 (2021/01/13)
 
